Switch over cons approach in flat
Begin unpicking previous work on adding constructors to flat
environment objects, and instead add constructor sibling
information to the pattern constructor elements themselves.
This should solve various headaches.

compiler/backend/flat_patternScript.sml
@@ -16,17 +16,10 @@ val _ = set_grammar_ancestry ["misc","flatLang","sptree",
     "pattern_semantics"];
 
 val _ = Datatype `config =
-  <| pat_heuristic : (* pattern_matching$branch list *) unit -> num ;
-    type_map : (num # num) list spt |>`;
-
-Definition init_type_map_def:
-  init_type_map = sptree$fromAList
-    [(bool_id, [(0 : num, 0 : num); (1, 0)]);
-        (1 (* list_id *), [(0, 0); (0, 2)])]
-End
+  <| pat_heuristic : (* pattern_matching$branch list *) unit -> num |>`;
 
 Definition init_config_def:
-  init_config ph = <| pat_heuristic := ph; type_map := init_type_map |>
+  init_config ph = <| pat_heuristic := ph |>
 End
 
 Definition sum_string_ords_def:
@@ -69,7 +62,7 @@ Definition compile_pat_bindings_def:
     (insert k () spt, Let t (SOME s) x exp2)) /\
   compile_pat_bindings t i ((Plit _, _, _) :: m) exp =
     compile_pat_bindings t i m exp /\
-  compile_pat_bindings t i ((Pcon stmp ps, k, x) :: m) exp = (
+  compile_pat_bindings t i ((Pcon _ ps, k, x) :: m) exp = (
     let j_nms = MAP (\(j, p). let k = i + 1 + j in
         let nm = enc_num_to_name k [] in
         ((j, nm), (p, k, Var_local t nm))) (enumerate 0 ps) in
@@ -146,16 +139,16 @@ Definition decode_dtree_def:
 End
 
 Definition encode_pat_def:
-  encode_pat type_map (flatLang$Pany) = pattern_semantics$Any /\
-  encode_pat type_map (Plit l) = Lit l /\
-  encode_pat type_map (Pvar _) = Any /\
-  encode_pat type_map (Pcon stmp ps) = Cons
+  encode_pat (flatLang$Pany) = pattern_semantics$Any /\
+  encode_pat (Plit l) = Lit l /\
+  encode_pat (Pvar _) = Any /\
+  encode_pat (flatLang$Pcon stmp ps) = Cons
     (case stmp of NONE => NONE | SOME (i, NONE) => SOME (i, NONE)
-        | SOME (i, SOME ty) => SOME (i, lookup ty type_map))
-    (MAP (encode_pat type_map) ps) /\
-  encode_pat type_map (Pref p) = Ref (encode_pat type_map p)
+        | SOME (i, SOME (ty, ctors)) => SOME (i, SOME ctors))
+    (MAP encode_pat ps) /\
+  encode_pat (Pref p) = Ref (encode_pat p)
 Termination
-  WF_REL_TAC `measure (pat_size o SND)`
+  WF_REL_TAC `measure pat_size`
   \\ rw [pat1_size]
   \\ fs [MEM_SPLIT, SUM_APPEND]
 End
@@ -194,7 +187,7 @@ Definition compile_pats_def:
   let branches = MAP (compile_pat_rhs t i v) ps in
   if naive then
   naive_pattern_matches t v (ZIP (MAP FST ps, branches)) default_x
-  else let pats = MAPi (\j (p, _). (encode_pat cfg.type_map p, j)) ps in
+  else let pats = MAPi (\j (p, _). (encode_pat p, j)) ps in
   let dt = pattern_comp$comp (* cfg.pat_heuristic *) pats
   in decode_dtree t (fromList branches) v default_x dt
 End
@@ -309,23 +302,9 @@ Proof
 QED
 
 Definition compile_dec_def:
-  compile_dec cfg (Dlet exp) =
-  (cfg, Dlet (SND (SND (compile_exp cfg exp))))
-  /\
-  compile_dec cfg (Dtype tid amap) =
-    (let new = FLAT (MAP (\(arity, max). MAP (\i. (i, arity)) (COUNT_LIST max))
-                (toAList amap)) in
-    (if NULL new then cfg
-        else cfg with type_map updated_by (insert tid new), Dtype tid amap)) /\
-  compile_dec cfg (Dexn n n') = (cfg, Dexn n n')
-End
-
-Definition compile_decs_def:
-  (compile_decs cfg [] = (cfg, [])) /\
-  (compile_decs cfg (d::ds) =
-    let (cfg1, e) = compile_dec cfg d in
-    let (cfg2, es) = compile_decs cfg1 ds in
-      (cfg2, e::es))
+  compile_dec cfg (Dlet exp) = Dlet (SND (SND (compile_exp cfg exp))) /\
+  compile_dec cfg (Dtype tid amap) = Dtype tid amap /\
+  compile_dec cfg (Dexn n n') = Dexn n n'
 End
 
 val _ = export_theory()
